Refactoring Header, Ctrl, and State to consolidate common parts of their proofs. (#23)
* Some progress on refactoring. Checkpointing to try some changes.

* Some more progress. The split screen technique works great!!

* Complete repair of the proof after refactoring.

Took longer than expected, and no actual lines of code savings yet, but the experience was still somewhat predictable, which is good.

* Some progress towards reducing lines of code by consolidating proofs.

Reduction is small with this commit, but it seems to at least be on the right track conceptually.

* Move things around to better organize lemmas.

* Start a typeclass.

* Finish generic proof of ptree_of_list

Still need to update specific proofs.

* Define an instance of CrVarLike for Header.

* Some thoughts on what else could be in the interface.

* WIP; doesn't work yet.

* Some more refactoring to consolidate proofs.

* Delete specific lemmas for state and header and use the generic one.

So much cleaner!

* Remove unnecessary record types for Headers/States/Ctrls from older commits.

Typeclasses are much simpler. And also avoid the need to change the sexpression format.

* Delete unused function.

* Attempt to minimize diff for code review.

* Remove more unnecessary things.

* First pass at unifying var equal definitions and lemmas

* added interface for retrieving maps from program state

* modified lookup/update argument order

* replaced update calls

* attempting to unify more CrProgramState lemmas

* Commit work with Sean to make a bit more progress.

* checkpoint

* Concrete to Symbolic Lemmas compiles

* compiles

* increment

* removed specific lookup/update calls

* unified more helpers

* removed dangling lemma

* more cleaning

* unified ps lookup lemmas

* simplified ProgramState record

* removed hdr/state soundness lemmas

* unify varlike comparison

* relocated generic helper lemma

* remove small redundancies

* remove unused lemma

* restore overeager removals

* Fix some code per Copilot review.

---------

Co-authored-by: seenry <s.rhee@nyu.edu>

CrConcreteSemanticsTransformer.v
@@ -24,10 +24,10 @@ Definition apply_bin_op (f : BinaryOp) (arg1 : uint8) (arg2 : uint8) : uint8 :=
 
 Definition lookup_concrete (arg : FunctionArgument) (ps : ConcreteState) : uint8 :=
   match arg with
-  | CtrlPlaneArg c => lookup_ctrl ps c
-  | HeaderArg h    => lookup_hdr ps h
+  | CtrlPlaneArg c => lookup_varlike_map (map_from_ps PSCtrl ps) c
+  | HeaderArg h    => lookup_varlike_map (map_from_ps PSHeader ps) h
   | ConstantArg n  => n
-  | StatefulArg s  => lookup_state ps s
+  | StatefulArg s  => lookup_varlike_map (map_from_ps PSState ps) s
   end.
 
 Definition eval_hdr_op_expr_concrete (op : HdrOp) (ps : ConcreteState) : uint8 :=
@@ -39,14 +39,14 @@ Definition eval_hdr_op_expr_concrete (op : HdrOp) (ps : ConcreteState) : uint8 :
 Definition eval_hdr_op_assign_concrete (op : HdrOp) (ps: ConcreteState) : ConcreteState :=
   match op with
   | StatefulOp f arg1 arg2 target =>
-        let op_output := eval_hdr_op_expr_concrete op ps in update_state ps target op_output
+        let op_output := eval_hdr_op_expr_concrete op ps in update_varlike PSState ps target op_output
   | StatelessOp f arg1 arg2 target => 
-        let op_output := eval_hdr_op_expr_concrete op ps in update_hdr ps target op_output
+        let op_output := eval_hdr_op_expr_concrete op ps in update_varlike PSHeader ps target op_output
   end.
 
 Definition eval_match_concrete (match_pattern : MatchPattern) (ps : ConcreteState) : bool :=
   (* For every list element, check if the Header's current value (determined by ps) equals the uint8 *)
-  List.forallb (fun '(h, v) => Integers.eq (lookup_hdr ps h) v) match_pattern.
+  List.forallb (fun '(h, v) => Integers.eq (lookup_varlike PSHeader ps h) v) match_pattern.
 
 (* Define evaluation over a list of HdrOp *)
 (* Note we are evaluating the list from right to left (fold_right) because it simplifies proving. *)
