CrProgramState.v
@@ -11,17 +11,12 @@ From Coq Require Import FunctionalExtensionality.
 Require Import Coq.Lists.List.
 Import ListNotations.
 
-(* Current values for each of these identifiers as a map *)
-Definition HeaderMap (T : Type) := PMap.t T. (* Maybe replace these with a generic Map type from Maps.v? *)
-Definition StateMap (T : Type) := PMap.t T.
-Definition CtrlMap (T : Type) := PMap.t T.
-
 (* The ProgramState is a record containing three maps:,
    one each for mapping headers/statevars/ctrlplaneconfigs to their current values *)
 Record ProgramState (T : Type) := {
-  ctrl_map : CtrlMap T;
-  header_map : HeaderMap T;
-  state_map : StateMap T;
+  ctrl_map : PMap.t T;
+  header_map : PMap.t T;
+  state_map : PMap.t T;
 }.
 
 Arguments header_map {T} _.
@@ -31,22 +26,193 @@ Arguments ctrl_map {T} _.
 Definition ConcreteState := ProgramState uint8.
 Definition SymbolicState := ProgramState SmtArithExpr.
 
-(* TODO: lookup_hdr/state_map could be rolled into lookup_hdr/state. *)
-(* TODO: It is used in a proof with a giant remember expression. *)
-Definition lookup_hdr_map {T : Type} (m: HeaderMap T) (x: Header) : T :=
-  PMap.get (match x with | HeaderCtr id => id end) m.
+Inductive PSField :=
+| PSCtrl
+| PSHeader
+| PSState.
 
-Definition lookup_state_map {T : Type} (m: StateMap T) (x: State) : T :=
-  PMap.get (match x with | StateCtr id => id end) m.
+Definition map_from_ps {T : Type} (field : PSField) (ps : ProgramState T) : PMap.t T :=
+  match field with
+  | PSCtrl => ctrl_map ps
+  | PSHeader => header_map ps
+  | PSState => state_map ps
+  end.
 
-Definition lookup_hdr {T : Type} (s: ProgramState T) (x: Header) : T :=
-  lookup_hdr_map (header_map s) x.
+Definition program_state_mapper {T1 T2 : Type} (fc: T1 -> T2) (fh : T1 -> T2) (fs : T1 -> T2) (s: ProgramState T1) : ProgramState T2 :=
+  {| ctrl_map := PMap.map fc (ctrl_map s);
+     header_map := PMap.map fh (header_map s);
+     state_map := PMap.map fs (state_map s) |}.
 
-Definition lookup_state {T : Type} (s: ProgramState T) (x: State) : T :=
-  lookup_state_map (state_map s) x.
+(* Function to go through all keys in a PMap, and set them to new values. *)
+Definition new_pmap_from_old {T: Type} (old_pmap : PMap.t T) (f : positive -> T): PMap.t T :=
+  (fst old_pmap, (* The old default value *)
+   PTree.map (fun x _ => f x) (snd old_pmap) (* Take old tree (snd old_pmap) and map elements from it (x) via function (f) *)
+  ).
 
-Definition lookup_ctrl {T : Type} (s: ProgramState T) (x: Ctrl) : T :=
-  PMap.get (match x with | CtrlCtr id => id end) (ctrl_map s).
+Definition lookup_varlike_map {T A : Type} `{CrVarLike A} (m : PMap.t T) (x : A) : T :=
+  PMap.get (get_key x) m.
+
+Definition lookup_varlike {T A : Type} `{CrVarLike A} (f: PSField) (s: ProgramState T) (x : A) : T :=
+  lookup_varlike_map (map_from_ps f s) x.
+
+Definition update_all_varlike {T A : Type} `{CrVarLike A} (f: PSField) (s: ProgramState T) (fh: A -> T) : ProgramState T :=
+  let new_map := new_pmap_from_old (map_from_ps f s) (fun pos => fh (make_item pos)) in
+  match f with
+  | PSCtrl =>   {| ctrl_map := new_map;
+                   header_map := header_map s;
+                   state_map := state_map s |}
+  | PSHeader => {| ctrl_map := ctrl_map s;
+                   header_map := new_map;
+                   state_map := state_map s |}
+  | PSState =>  {| ctrl_map := ctrl_map s;
+                   header_map := header_map s;
+                   state_map := new_map |}
+  end.
+
+Definition update_varlike_map {T A : Type} `{CrVarLike A} (m: PMap.t T) (x: A) (v: T) : PMap.t T :=
+  PMap.set (get_key x) v m.
+  
+Definition update_varlike {T A : Type} `{CrVarLike A} (f: PSField) (s: ProgramState T) (x: A) (v: T) : ProgramState T :=
+  let new_map := update_varlike_map (map_from_ps f s) x v in
+  match f with
+  | PSCtrl =>   {| ctrl_map := new_map;
+                   header_map := header_map s;
+                   state_map := state_map s |}
+  | PSHeader => {| ctrl_map := ctrl_map s;
+                   header_map := new_map;
+                   state_map := state_map s |}
+  | PSState =>  {| ctrl_map := ctrl_map s;
+                   header_map := header_map s;
+                   state_map := new_map |}
+  end.
+
+Lemma update_all_varlike_lookup_unchanged:
+  forall {T A} `{CrVarLike A} (s1 : ProgramState T) (f : PSField),
+   update_all_varlike f s1 (fun v : A => lookup_varlike_map (map_from_ps f s1) v) = s1.
+Proof.
+  intros.
+  destruct s1 as [ctrl hdr state].
+  unfold update_all_varlike.
+  destruct f;
+  simpl;
+  f_equal; try reflexivity;
+  unfold lookup_varlike_map;
+  unfold new_pmap_from_old;
+  simpl;
+  try destruct ctrl; try destruct hdr; try destruct state;
+  simpl;
+  f_equal;
+  apply PTree.extensionality;
+  intros;
+  rewrite PTree.gmap;
+  unfold Coqlib.option_map;
+  unfold PMap.get;
+  simpl;
+  rewrite inverses'.
+  - destruct (t0 ! i) eqn:des; auto.
+  - destruct (t2 ! i) eqn:des; auto.
+  - destruct (t4 ! i) eqn:des; auto.
+Qed.
+
+Lemma commute_lookup_varlike:
+  forall {T1 T2 A} `{CrVarLike A} ps v (func : T1 -> T2) f,
+  lookup_varlike f (program_state_mapper func func func ps) v =
+  func (lookup_varlike_map (map_from_ps f ps) v).
+Proof.
+  intros.
+  destruct f;
+  apply PMap.gmap.
+Qed.
+
+Lemma commute_mapper_update_varlike:
+  forall {T1 T2 A} `{CrVarLike A} ps x v (func : T1 -> T2) f,
+  program_state_mapper func func func (update_varlike f ps x v) =
+  update_varlike f (program_state_mapper func func func ps) x (func v).
+Proof.
+  intros.
+  unfold program_state_mapper.
+  unfold update_varlike.
+  destruct f;
+  f_equal;
+  simpl;
+  unfold update_varlike_map;
+  destruct ps;
+  simpl;
+  unfold PMap.set;
+  unfold PMap.map;
+  simpl;
+  f_equal;
+  apply PTree.extensionality;
+  intros;
+  simpl;
+  rewrite PTree.gsspec;
+  rewrite PTree.gmap1;
+  rewrite PTree.gsspec.
+  1-3: destruct (Coqlib.peq i (get_key x));
+  try subst; try reflexivity;
+  try rewrite PTree.gmap1; try reflexivity.
+Qed.
+
+Lemma lookup_f1_unchanged_by_update_all_f2:
+  forall {T A} `{CrVarLike A} fs (s1 : ProgramState T) (h : A) f1 f2,
+  f1 <> f2 ->
+    lookup_varlike_map (map_from_ps f1 s1) h =
+    lookup_varlike_map (map_from_ps f1 (update_all_varlike f2 s1 fs)) h.
+Proof.
+  intros.
+  destruct f1, f2;
+  try reflexivity;
+  try congruence.
+Qed.
+
+Definition is_varlike_in_ps {T A} `{CrVarLike A} (f : PSField) (s1 : ProgramState T) (v : A) :=
+  PTree.get (get_key v) (snd (map_from_ps f s1)).
+
+Lemma lookup_varlike_after_update_all_varlike:
+  forall {T A} `{CrVarLike A} (s1 : ProgramState T) (v : A) (fv : A -> T) field,
+    is_varlike_in_ps field s1 v <> None ->
+    lookup_varlike_map (map_from_ps field (update_all_varlike field s1 fv)) v = fv v.
+Proof.
+  intros.
+  unfold lookup_varlike_map.
+  unfold update_all_varlike.
+  destruct field;
+  simpl;
+  unfold lookup_varlike_map;
+  unfold new_pmap_from_old;
+  simpl;
+  unfold is_varlike_in_ps in H0; simpl in H0;
+  try destruct (map_from_ps PSCtrl s1) as [default ctrl];
+  try destruct (map_from_ps PSHeader s1) as [default header];
+  try destruct (map_from_ps PSState s1) as [default state];
+  unfold PMap.get;
+  simpl;
+  rewrite PTree.gmap;
+  unfold Coqlib.option_map;
+  rewrite inverses;
+  simpl;
+  simpl in H.
+  - destruct (snd (ctrl_map s1)) ! (get_key v) eqn:des. auto. congruence.
+  - destruct (snd (header_map s1)) ! (get_key v) eqn:des. try auto. congruence.
+  - destruct (snd (state_map s1)) ! (get_key v) eqn:des. try auto. congruence.
+Qed.
+
+Lemma commute_varlike_updates:
+  forall {T A A'}
+    `{CrVarLike A}
+    `{CrVarLike A'}
+    (s1 : ProgramState T)
+    (f f' : PSField)
+    (fv : A -> T) (fv' : A' -> T),
+  f <> f' ->
+    update_all_varlike f (update_all_varlike f' s1 fv') fv =
+    update_all_varlike f' (update_all_varlike f s1 fv) fv'.
+Proof.
+  intros.
+  destruct f, f';
+  try congruence;
+  try unfold update_all_varlike; f_equal.
+Qed.
 
 Lemma program_state_equality:
       forall (ps1 ps2: ConcreteState),
@@ -62,384 +228,53 @@ Proof.
   f_equal; try assumption.
 Qed.
 
-Definition program_state_mapper {T1 T2 : Type} (fc: T1 -> T2) (fh : T1 -> T2) (fs : T1 -> T2) (s: ProgramState T1) : ProgramState T2 :=
-  {| ctrl_map := PMap.map fc (ctrl_map s);
-     header_map := PMap.map fh (header_map s);
-     state_map := PMap.map fs (state_map s) |}.
-
-(* Function to go through all keys in a PMap, and set them to new values. *)
-Definition new_pmap_from_old {T: Type} (old_pmap : PMap.t T) (f : positive -> T): PMap.t T :=
-  (fst old_pmap, (* The old default value *)
-   PTree.map (fun x _ => f x) (snd old_pmap) (* Take old tree (snd old_pmap) and map elements from it (x) via function (f) *)
-  ).
-
-Definition update_all_hdrs {T : Type} (s: ProgramState T) (fh: Header -> T) : ProgramState T :=
-  {| ctrl_map := ctrl_map s;
-     header_map := new_pmap_from_old (header_map s) (fun pos => fh (HeaderCtr pos));
-     state_map := state_map s |}.
-
-Definition update_all_states {T : Type} (s: ProgramState T) (fs: State -> T) : ProgramState T :=
-  {| ctrl_map := ctrl_map s;
-     header_map := header_map s;
-     state_map := new_pmap_from_old (state_map s) (fun pos => fs (StateCtr pos))|}.
-
-(* Update the header map with a new value for a specific header *)
-Definition update_hdr_map {T : Type} (m: HeaderMap T) (x: Header) (v: T) : HeaderMap T :=
-  PMap.set (match x with | HeaderCtr x_id => x_id end) v m.
-
-(* Same as above, but for state variables *)
-Definition update_state_map {T : Type} (m: StateMap T) (x: State) (v: T) : StateMap T :=
-  PMap.set (match x with | StateCtr x_id => x_id end) v m.
-
-Definition update_hdr {T : Type} (s: ProgramState T) (x: Header) (v: T) : ProgramState T :=
-  {|ctrl_map :=ctrl_map s;
-     header_map :=  update_hdr_map (header_map s) x v;
-     state_map := state_map s|}.
-
-Definition update_state {T : Type} (s: ProgramState T) (x: State) (v: T) : ProgramState T :=
-  {|ctrl_map :=ctrl_map s;
-     header_map := header_map s;
-     state_map := update_state_map (state_map s) x v |}.
-
-Lemma cons_not_nil : forall A (x : A) (xs : list A),
-  ~ ((x :: xs) = nil).
-Proof.
-  intros.
-  simpl.
-  unfold "<>".
-  intros.
-  discriminate H.
-Qed.
-
-Lemma update_all_hdrs_lookup_unchanged:
-  forall {T} (s1 : ProgramState T),
-   update_all_hdrs s1 (fun h : Header => lookup_hdr s1 h) = s1.
-Proof.
-  intros.
-  destruct s1 as [ctrl hdr state].
-  unfold update_all_hdrs.
-  simpl.
-  f_equal; try reflexivity.
-  unfold lookup_hdr.
-  simpl.
-  unfold lookup_hdr_map.
-  unfold new_pmap_from_old.
-  simpl.
-  destruct hdr.
-  simpl.
-  f_equal.
-  apply PTree.extensionality.
-  intros.
-  rewrite PTree.gmap.
-  unfold Coqlib.option_map.
-  unfold PMap.get.
-  simpl.
-  destruct (t0 ! i) eqn:des; auto.
-Qed.
-
-(* Same lemma as above but for state *)
-Lemma update_all_states_lookup_unchanged:
-  forall {T} (s1 : ProgramState T),
-   update_all_states s1 (fun sv : State => lookup_state s1 sv) = s1.
-Proof.
-  intros.
-  destruct s1 as [ctrl hdr state].
-  unfold update_all_states.
-  simpl.
-  f_equal; try reflexivity.
-  unfold lookup_state.
-  simpl.
-  unfold lookup_state_map.
-  unfold new_pmap_from_old.
-  simpl.
-  destruct state.
-  simpl.
-  f_equal.
-  apply PTree.extensionality.
-  intros.
-  rewrite PTree.gmap.
-  unfold Coqlib.option_map.
-  unfold PMap.get.
-  simpl.
-  destruct (t0 ! i) eqn:des; auto.
-Qed.
-
 Lemma program_state_unchanged:
   forall {T} (s1 : ProgramState T),
-  update_all_states (update_all_hdrs s1 (fun h : Header => lookup_hdr s1 h))
-                    (fun s : State => lookup_state s1 s) = s1.
+  update_all_varlike PSState (update_all_varlike PSHeader s1 (fun h : Header => lookup_varlike_map (map_from_ps PSHeader s1) h))
+                    (fun s : State => lookup_varlike_map (map_from_ps PSState s1) s) = s1.
 Proof.
   intros.
-  rewrite update_all_hdrs_lookup_unchanged.
-  rewrite update_all_states_lookup_unchanged.
-  reflexivity.
-Qed.        
-
-Lemma commute_mapper_lookup_ctrl:
-  forall {T1} {T2} ps c (func : T1 -> T2),
-  lookup_ctrl (program_state_mapper func func func ps) c =
-  func (lookup_ctrl ps c).
-Proof.
-  intros.
-  apply PMap.gmap.
-Qed.
-
-Lemma commute_mapper_lookup_state:
-  forall {T1} {T2} ps sv (func : T1 -> T2),
-  lookup_state (program_state_mapper func func func ps) sv =
-  func (lookup_state ps sv).
-Proof.
-  intros.
-  apply PMap.gmap.
-Qed.
-
-Lemma commute_mapper_lookup_hdr:
-  forall {T1} {T2} ps hv (func : T1 -> T2),
-  lookup_hdr (program_state_mapper func func func ps) hv =
-  func (lookup_hdr ps hv).
-Proof.
-  intros.
-  apply PMap.gmap.
-Qed.
-
-Lemma commute_mapper_update_hdr:
-  forall {T1} {T2} ps h v (func : T1 -> T2),
-  program_state_mapper func func func (update_hdr ps h v) =
-  update_hdr (program_state_mapper func func func ps) h (func v).
-Proof.
-  intros.
-  unfold program_state_mapper.
-  unfold update_hdr.
-  f_equal.
-  simpl.
-  unfold update_hdr_map.
-  destruct ps.
-  simpl.
-  destruct h. simpl.
-  unfold PMap.set.
-  unfold PMap.map.
-  simpl.
-  f_equal.
-  apply PTree.extensionality.
-  intros.
-  simpl.
-  rewrite PTree.gsspec.
-  rewrite PTree.gmap1.
-  rewrite PTree.gsspec.
-  destruct (Coqlib.peq i uid).
-  - subst. reflexivity.
-  - rewrite PTree.gmap1.
-    reflexivity.
-Qed.
-
-Lemma commute_mapper_update_state:
-  forall {T1} {T2} ps sv v (func : T1 -> T2),
-  program_state_mapper func func func (update_state ps sv v) =
-  update_state (program_state_mapper func func func ps) sv (func v).
-Proof.
-  intros.
-  unfold program_state_mapper.
-  unfold update_state.
-  f_equal.
-  simpl.
-  unfold update_state_map.
-  destruct ps.
-  simpl.
-  destruct sv. simpl.
-  unfold PMap.set.
-  unfold PMap.map.
-  simpl.
-  f_equal.
-  apply PTree.extensionality.
-  intros.
-  simpl.
-  rewrite PTree.gsspec.
-  rewrite PTree.gmap1.
-  rewrite PTree.gsspec.
-  destruct (Coqlib.peq i uid).
-  - subst. reflexivity.
-  - rewrite PTree.gmap1.
-    reflexivity.
-Qed.
-
-Lemma lookup_hdr_unchanged_by_update_all_states:
-  forall {T} fs (s1 : ProgramState T) (h : Header),
-    lookup_hdr s1 h = lookup_hdr (update_all_states s1 fs) h.
-Proof.
+  repeat rewrite update_all_varlike_lookup_unchanged.
   reflexivity.
 Qed.
 
-Definition is_header_in_ps {T} (s1 : ProgramState T) (h : Header) :=
-  PTree.get (match h with | HeaderCtr id => id end) (snd (header_map s1)).
-
-Lemma lookup_hdr_after_update_all_hdrs:
-  forall {T} (s1 : ProgramState T) (h : Header) (fh : Header -> T),
-    is_header_in_ps s1 h <> None ->
-    lookup_hdr (update_all_hdrs s1 fh) h = fh h.
+Lemma is_v1_in_ps_after_update_all_v2:
+  forall {T A A'} `{CrVarLike A} `{CrVarLike A'} (s1 : ProgramState T)
+    f1 f2 (h : A) (fs : A' -> T),
+    f1 <> f2 ->
+    is_varlike_in_ps f1 (update_all_varlike f2 s1 fs) h = is_varlike_in_ps f1 s1 h.
 Proof.
   intros.
-  unfold lookup_hdr.
-  unfold update_all_hdrs.
-  simpl.
-  unfold lookup_hdr_map.
-  unfold new_pmap_from_old.
-  simpl.
-  unfold is_header_in_ps in H.
-  destruct (header_map s1) as [default hdr].
-  simpl.
-  f_equal.
-  unfold PMap.get.
-  simpl.
-  rewrite PTree.gmap.
-  unfold Coqlib.option_map.
-  destruct h.
-  simpl.
-  simpl in H.
-  destruct (hdr ! uid) eqn:des; auto.
-  congruence.
-Qed.
-
-(* Create mirror image versions of the two lemmas above with state and hdr interchanged *)
-Lemma lookup_state_unchanged_by_update_all_hdrs:
-  forall {T} fh (s1 : ProgramState T) (sv : State),
-    lookup_state s1 sv = lookup_state (update_all_hdrs s1 fh) sv.
-Proof.
+  destruct f1, f2; try congruence;
   reflexivity.
 Qed.
 
-Definition is_state_var_in_ps {T} (s1 : ProgramState T) (sv : State) :=
-  PTree.get (match sv with | StateCtr id => id end) (snd (state_map s1)).
+Definition get_all_varlike_from_ps {T A : Type} `{CrVarLike A} (f : PSField) (s: ProgramState T) : list A :=
+  List.map (fun '(key, value) => make_item key)
+           (PTree.elements (snd (map_from_ps f s))).
 
-Lemma lookup_state_after_update_all_states:
-  forall {T} (s1 : ProgramState T) (sv : State) (fs : State -> T),
-    is_state_var_in_ps s1 sv <> None ->
-    lookup_state (update_all_states s1 fs) sv = fs sv.
+Lemma is_varlike_in_ps_lemma :
+  forall {T A} `{CrVarLike A} (f : PSField) (s1 : ProgramState T) (v : A),
+    In v (get_all_varlike_from_ps f s1) ->
+    is_varlike_in_ps f s1 v <> None.
 Proof.
-  intros.
-  unfold lookup_state.
-  unfold update_all_states.
-  simpl.
-  unfold lookup_state_map.
-  unfold new_pmap_from_old.
-  simpl.
-  unfold is_state_var_in_ps in H.
-  destruct (state_map s1) as [default sv_map].
-  simpl.
-  f_equal.
-  unfold PMap.get.
-  simpl.
-  rewrite PTree.gmap.
-  unfold Coqlib.option_map.
-  destruct sv.
-  simpl.
-  simpl in H.
-  destruct (sv_map ! uid) eqn:des; auto.
-  congruence.
-Qed.
-
-Lemma commute_state_hdr_updates:
-  forall {T} (s1 : ProgramState T) (fh : Header -> T) (fs : State -> T),
-    update_all_hdrs (update_all_states s1 fs) fh =
-    update_all_states (update_all_hdrs s1 fh) fs.
-Proof.
-  reflexivity.
-Qed.
-
-Lemma lookup_hdr_trivial:
-  forall {T} (s : ProgramState T) (h : Header),
-    lookup_hdr s h = lookup_hdr_map (header_map s) h.
-Proof.
-  intros.
-  reflexivity.
-Qed.
-
-Lemma lookup_state_trivial:
-  forall {T} (s : ProgramState T) (sv : State),
-    lookup_state s sv = lookup_state_map (state_map s) sv.
-Proof.
-  intros.
-  reflexivity.
-Qed.
-
-(* is_header_in_ps is preserved across update_all_states *)
-Lemma is_header_in_ps_after_update_all_states:
-  forall {T} (s1 : ProgramState T) (h : Header) (fs : State -> T),
-    is_header_in_ps (update_all_states s1 fs) h = is_header_in_ps s1 h.
-Proof.
-  intros.
-  reflexivity.
-Qed.
-
-(* is_state_var_in_ps is preserved across update_all_hdrs *)
-Lemma is_state_var_in_ps_after_update_all_hdrs:
-  forall {T} (s1 : ProgramState T) (sv : State) (fh : Header -> T),
-    is_state_var_in_ps (update_all_hdrs s1 fh) sv = is_state_var_in_ps s1 sv.
-Proof.
-  intros.
-  reflexivity.
-Qed.
-
-Definition get_all_headers_from_ps {T : Type} (s: ProgramState T) : list Header :=
-  List.map (fun '(key, value) => HeaderCtr key)
-           (PTree.elements (snd (header_map s))).
-
-Definition get_all_states_from_ps {T : Type} (s: ProgramState T) : list State :=
-  List.map (fun '(key, value) => StateCtr key)
-           (PTree.elements (snd (state_map s))).
-
-Definition get_all_ctrls_from_ps {T : Type} (s: ProgramState T) : list Ctrl :=
-  List.map (fun '(key, value) => CtrlCtr key)
-           (PTree.elements (snd (ctrl_map s))).
-
-Lemma is_header_in_ps_lemma :
-  forall {T} (s1 : ProgramState T) (h : Header),
-    In h (get_all_headers_from_ps s1) ->
-    is_header_in_ps s1 h <> None.
-    (* TODO: Need to ask Joe about <> None *)
-Proof.
-  intros.
+  intros T A HA f s1 v H.
   destruct s1 as [ctrl hdr state].
-  unfold get_all_headers_from_ps in H.
-  unfold is_header_in_ps.
-  simpl in *.
-  destruct hdr as [default hdr_map].
-  simpl in *.
-  apply in_map_iff in H.
-  simpl in H.
-  destruct H. (* TODO: ask Joe, seems to extract witness *)
-  destruct x.
-  destruct h.
-  destruct H.
-  injection H as H_eq.
-  rewrite <- H_eq.
-  apply some_is_not_none with (x := t).
-  apply PTree.elements_complete.
-  assumption.
-Qed.
-
-(* Same as above lemma, but for state *)
-Lemma is_state_in_ps_lemma :
-  forall {T} (s1 : ProgramState T) (sv : State),
-    In sv (get_all_states_from_ps s1) ->
-    is_state_var_in_ps s1 sv <> None.
-Proof.
-  intros.
-  destruct s1 as [ctrl hdr state].
-  unfold get_all_states_from_ps in H.
-  unfold is_state_var_in_ps.
-  simpl in *.
-  destruct state as [default state_map].
-  simpl in *.
-  apply in_map_iff in H.
-  simpl in H.
-  destruct H. (* TODO: ask Joe, seems to extract witness *)
-  destruct x.
-  destruct sv.
-  destruct H.
-  injection H as H_eq.
-  rewrite <- H_eq.
-  apply some_is_not_none with (x := t).
-  apply PTree.elements_complete.
+  destruct f;
+  unfold get_all_varlike_from_ps in H;
+  unfold is_varlike_in_ps;
+  simpl in *;
+  destruct ctrl as [c0 ctrl_map];
+  destruct hdr as [h0 hdr_map];
+  destruct state as [s0 state_map];
+  simpl in *;
+  apply in_map_iff in H;
+  destruct H; (* TODO: ask Joe, seems to extract witness *)
+  destruct x;
+  destruct H;
+  rewrite <- H; rewrite inverses';
+  apply some_is_not_none with (x := t);
+  apply PTree.elements_complete;
   assumption.
 Qed.
 
@@ -447,15 +282,15 @@ Definition init_concrete_state (p : CaracaraProgram) : ConcreteState :=
   let h := get_headers_from_prog p in
   let s := get_states_from_prog p in
   let c := get_ctrls_from_prog p in
-  {|ctrl_map :=  (repr 0, (* TODO: Need better default, but think this doesn't matter *)
-                        PTree_Properties.of_list
-                        (List.map (fun x => (match x with | CtrlCtr x_id => x_id end, repr 0)) c));
-     header_map     :=  (repr 0, (* TODO: Need better default, but think this doesn't matter *)
-                        PTree_Properties.of_list
-                        (List.map (fun x => (match x with | HeaderCtr x_id => x_id end, repr 0)) h));
+  {|ctrl_map    :=  (repr 0, (* TODO: Need better default, but think this doesn't matter *)
+                    PTree_Properties.of_list
+                    (List.map (fun x => (match x with | CtrlCtr x_id => x_id end, repr 0)) c));
+     header_map :=  (repr 0, (* TODO: Need better default, but think this doesn't matter *)
+                    PTree_Properties.of_list
+                    (List.map (fun x => (match x with | HeaderCtr x_id => x_id end, repr 0)) h));
      state_map  :=  (repr 0,
-                        PTree_Properties.of_list
-                        (List.map (fun x => (match x with | StateCtr x_id => x_id end, repr 0)) s));|}.
+                    PTree_Properties.of_list
+                    (List.map (fun x => (match x with | StateCtr x_id => x_id end, repr 0)) s));|}.
 
 (* Convert positive to string *)
 Fixpoint pos_to_string (p : positive) : string :=
@@ -481,28 +316,14 @@ Definition init_symbolic_state (p: CaracaraProgram) : SymbolicState :=
 
 Definition is_init_state {T} (p : CaracaraProgram) (ps : ProgramState T) : Prop :=
   forall h sv c,
-    (In h (get_headers_from_prog p) <-> In h (get_all_headers_from_ps ps)) /\
-    (In sv (get_states_from_prog p) <-> In sv (get_all_states_from_ps ps)) /\
-    (In c (get_ctrls_from_prog p) <-> In c (get_all_ctrls_from_ps ps)).
+    (In h (get_headers_from_prog p) <-> In h (get_all_varlike_from_ps PSHeader ps)) /\
+    (In sv (get_states_from_prog p) <-> In sv (get_all_varlike_from_ps PSState ps)) /\
+    (In c (get_ctrls_from_prog p) <-> In c (get_all_varlike_from_ps PSCtrl ps)).
 
 (* Mark definitions globally opaque below *)
-Global Opaque lookup_ctrl.
-Global Opaque update_hdr_map.
-Global Opaque update_state_map.
-Global Opaque update_hdr.
-Global Opaque update_state.
-Global Opaque lookup_hdr.
-Global Opaque lookup_state.
-Global Opaque lookup_hdr_map.
-Global Opaque lookup_state_map.
+Global Opaque update_varlike_map.
+Global Opaque lookup_varlike_map.
 Global Opaque program_state_mapper.
-Global Opaque update_all_hdrs.
-Global Opaque update_all_states.
-Global Opaque HeaderMap.
-Global Opaque StateMap.
-Global Opaque CtrlMap.
 Global Opaque new_pmap_from_old.
-Global Opaque is_header_in_ps.
-Global Opaque is_state_var_in_ps.
-Global Opaque get_all_headers_from_ps.
-Global Opaque get_all_states_from_ps.
+Global Opaque get_all_varlike_from_ps.
+Global Opaque map_from_ps.
