HelperLemmas.v
@@ -12,29 +12,16 @@ From MyProject Require Import PMapHelperLemmas.
 From MyProject Require Import CrProgramState.
 From MyProject Require Import ListUtils.
 
-Lemma commute_lookup_eval_state:
-  forall (s : SymbolicState) (f : SmtValuation)
-        sv,
-    lookup_state (eval_sym_state s f) sv =
-    eval_smt_arith (lookup_state s sv) f.
+Lemma commute_lookup_eval_varlike:
+  forall {A} `{CrVarLike A} (field : PSField) (ps : SymbolicState)
+        (var : A) (val : SmtValuation),
+    lookup_varlike field (eval_sym_state ps val) var =
+    eval_smt_arith (lookup_varlike field ps var) val.
 Proof.
-  intros s f sv.
-  destruct sv.
-  unfold eval_sym_state.
-  rewrite commute_mapper_lookup_state.
-  reflexivity.
-Qed.
-
-Lemma commute_lookup_eval_hdr:
-  forall (s : SymbolicState) (f : SmtValuation)
-        hv,
-    lookup_hdr (eval_sym_state s f) hv =
-    eval_smt_arith (lookup_hdr s hv) f.
-Proof.
-  intros s f hv.
-  destruct hv.
-  unfold eval_sym_state.
-  rewrite commute_mapper_lookup_hdr.
+  intros.
+  destruct field;
+  unfold eval_sym_state;
+  rewrite commute_lookup_varlike;
   reflexivity.
 Qed.
 
@@ -45,10 +32,9 @@ Lemma commute_lookup_eval:
     eval_smt_arith (lookup_smt arg s) f.
 Proof.
   intros s f arg.
-  destruct arg; simpl; try reflexivity.
-  -- unfold eval_sym_state. rewrite commute_mapper_lookup_ctrl. reflexivity.
-  -- unfold eval_sym_state. rewrite commute_mapper_lookup_hdr. reflexivity.
-  -- unfold eval_sym_state. rewrite commute_mapper_lookup_state. reflexivity.
+  unfold lookup_concrete.
+  destruct arg; simpl; try reflexivity;
+  apply commute_lookup_eval_varlike.
 Qed.
 
 Lemma find_first_match_lemma:
@@ -83,27 +69,4 @@ Proof.
     -- inversion H. left. reflexivity.
     -- right. apply IHrest.
        assumption.
-Qed.
-
-Lemma header_map_ps : (*TODO: Should probably be called lookup_hdr_ps *)
-  forall s f h,
-    lookup_hdr (eval_sym_state s f) h =
-    eval_smt_arith (lookup_hdr s h) f.
-Proof.
-  intros.
-  unfold eval_sym_state.
-  rewrite commute_mapper_lookup_hdr.
-  reflexivity.
-Qed.
-
-(* Create a lemma similar to header_map_ps but with state_var_map instead *)
-Lemma state_var_map_ps : (* Same TODO as header_map_ps, bad naming *)
-  forall s f sv,
-    lookup_state (eval_sym_state s f) sv =
-    eval_smt_arith (lookup_state s sv) f.
-Proof.
-  intros.
-  unfold eval_sym_state.
-  rewrite commute_mapper_lookup_state.
-  reflexivity.
 Qed.
