PMapHelperLemmas.v
@@ -2,42 +2,63 @@ From MyProject Require Import SmtExpr.
 From MyProject Require Import CrProgramState.
 From MyProject Require Import CrSymbolicSemanticsTransformer.
 From MyProject Require Import Maps.
+From MyProject Require Import UtilLemmas.
+From MyProject Require Import CrIdentifiers.
+Require Import Coq.Lists.List.
+Require Import ZArith.
 
-Transparent lookup_ctrl.
-Lemma commute_lookup_eval_ctrl:
-  forall c f s,
-  lookup_ctrl (eval_sym_state s f) c =
-  eval_smt_arith (lookup_ctrl s c) f.
+Transparent map_from_ps.
+Transparent lookup_varlike_map.
+Lemma commute_lookup_eval_generic:
+  forall (A: Type) `{CrVarLike A} (v : A) field_type f ps,
+  lookup_varlike_map (map_from_ps field_type (eval_sym_state ps f)) v =
+  eval_smt_arith (lookup_varlike_map (map_from_ps field_type ps) v) f.
 Proof.
   intros.
-  apply PMap.gmap.
+  unfold map_from_ps.
+  destruct field_type; simpl; apply PMap.gmap.
 Qed.
 
 (* Same as the above lemma for hdr and state *)
-Transparent lookup_hdr.
-Transparent lookup_hdr_map.
-Lemma commute_lookup_eval_hdr:
-  forall h f s,
-  lookup_hdr (eval_sym_state s f) h =
-  eval_smt_arith (lookup_hdr s h) f.
+Lemma ptree_of_list_lemma_generic:
+    forall (X : Type) `(CrVarLike X)
+    (l : list X) (val_fn : X -> SmtArithExpr)
+    (x : X),
+    Coqlib.list_norepet l ->
+    In x l ->
+    In x (map (fun '(key, _) => make_item key)
+    (PTree.elements (PTree_Properties.of_list (combine (map get_key l) (map val_fn l))))).
 Proof.
+  intros X crvarlike l val_fn x H' H.
+  generalize H as H_in.
+  apply functional_list_helper with (key_fn := get_key) (val_fn := val_fn) in H.
   intros.
-  apply PMap.gmap.
+  remember (fun '(key, _) => make_item key) as f.
+  assert(H_tmp: x =
+          f (get_key x, val_fn (x))). {
+  rewrite Heqf.
+  rewrite (inverses x).
+  reflexivity. }
+  rewrite H_tmp.
+  apply in_map with (f := f) (x := (get_key x, val_fn x)) (l := (PTree.elements
+  (PTree_Properties.of_list (combine (map get_key l) (map val_fn l))))).
+  remember (get_key x, val_fn x) as pair_val.
+  remember (combine (map get_key l) (map val_fn l)) as l_combined.
+  rewrite Heqpair_val in *.
+  apply PTree.elements_correct with (m := PTree_Properties.of_list l_combined).
+  apply PTree_Properties.of_list_norepet.
+  - rewrite Heql_combined.
+    simpl.
+    rewrite map_combine2.
+    apply Coqlib.list_map_norepet.
+    -- assumption.
+    -- intros.
+       apply (inj x0 y).
+       assumption.
+  - simpl in H. rewrite Heqf in H_tmp.
+    rewrite H_tmp.
+    rewrite inverses.
+    assumption.
 Qed.
 
-Transparent lookup_state.
-Transparent lookup_state_map.
-Lemma commute_lookup_eval_state:
-  forall sv f s,
-  lookup_state (eval_sym_state s f) sv =
-  eval_smt_arith (lookup_state s sv) f.
-Proof.
-  intros.
-  apply PMap.gmap.
-Qed.
-
-Global Opaque lookup_hdr.
-Global Opaque lookup_state.
-Global Opaque lookup_hdr_map.
-Global Opaque lookup_state_map.
-Global Opaque lookup_ctrl.
+Global Opaque lookup_varlike_map.
